coq/Translation/CAMPRuletoCAMP.v
@@ -1,0 +1,49 @@
+(*
+ * Copyright 2015-2016 IBM Corporation
+ *
+ * Licensed under the Apache License, Version 2.0 (the "License");
+ * you may not use this file except in compliance with the License.
+ * You may obtain a copy of the License at
+ *
+ * http://www.apache.org/licenses/LICENSE-2.0
+ *
+ * Unless required by applicable law or agreed to in writing, software
+ * distributed under the License is distributed on an "AS IS" BASIS,
+ * WITHOUT WARRANTIES OR CONDITIONS OF ANY KIND, either express or implied.
+ * See the License for the specific language governing permissions and
+ * limitations under the License.
+ *)
+
+Section CAMPRuletoCAMP.
+
+  Require Import String.
+  Require Import List.
+
+  Require Import Utils BasicRuntime.
+  Require Import CAMPRuleRuntime.
+  Require Import CAMPRuntime.
+  
+  Section Top.
+    Context {fr:foreign_runtime}.
+    (** Note: Translation from CAMP Rules to CAMP is really macro-expansion *)
+    Definition camp_rule_to_camp_top (q:camp_rule) : camp := camp_rule_to_camp q.
+
+    Context (h:brand_relation_t).
+
+    Theorem camp_rule_to_camp_top_correct :
+      forall q:camp_rule, forall global_env:bindings,
+          camp_rule_eval_top h q global_env =
+          camp_eval_top h (camp_rule_to_camp_top q) global_env.
+    Proof.
+      intros.
+      reflexivity.
+    Qed.
+  End Top.
+    
+End CAMPRuletoCAMP.
+
+(* 
+*** Local Variables: ***
+*** coq-load-path: (("../../coq" "Qcert")) ***
+*** End: ***
+*)
